add alpha blending spec

RL.v
@@ -1,6 +1,6 @@
 Set Implicit Arguments.
 From SLF Require Import LabType Fun LibSepFmap Sum.
-From SLF Require Import LibWP LibSepSimpl LibSepReference LibSepTLCbuffer Struct Loops Unary.
+From SLF Require Import LibWP LibSepSimpl LibSepReference LibSepTLCbuffer Struct Loops Unary ListCommon.
 From mathcomp Require Import ssreflect ssrfun zify.
 Hint Rewrite conseq_cons' : rew_listx.
 
@@ -17,14 +17,28 @@ Coercion to_int : val >-> Z.
 
 Module runlength.
 
-(* FIXME: A possible problem is that search assumes the existence of answer, while index does not;
-    this may be bad. 
-  As a direct result, only one spec of rli is proven. *)
+Notation "'for' i <- '[' Z ',' N ']' '{' t '}'"  :=
+  (For Z N <{ fun_ i => t }>)
+  (in custom trm at level 69,
+    Z, N, i at level 0,
+    format "'[' for  i  <-  [ Z ','  N ] ']'  '{' '/   ' '[' t  '}' ']'") : trm_scope.
 
-Section runlength.
+Notation "'while' C '{' T '}'"  :=
+  (While C T)
+  (in custom trm at level 69,
+    C, T at level 0,
+    format "'[' while  C ']'  '{' '/   ' '[' T  '}' ']'") : trm_scope.
 
 Notation "'xind'" := ("x_ind":var) (in custom trm at level 0) : trm_scope.
 Notation "'xval'" := ("x_val":var) (in custom trm at level 0) : trm_scope.
+Notation "'yind'" := ("y_ind":var) (in custom trm at level 0) : trm_scope.
+Notation "'yval'" := ("y_val":var) (in custom trm at level 0) : trm_scope.
+
+(* FIXME: A possible problem is that search assumes the existence of answer, while index does not;
+    this may be bad. 
+  As a direct result, only one spec of get is proven. *)
+
+Section runlength.
 
 Import List Vars.
 
@@ -36,22 +50,22 @@ Local Notation D := (labeled int).
 
 Implicit Type d : D.
 
-Section rli.
+Section get.
 
-Definition rli := 
+Definition get := 
   <{
   fun i xind xval =>
     let k = search.func i xind in 
     read_array xval k
 }>.
 
-Lemma rli_spec_unary `{Inhab D} (x_ind x_val : loc) d 
+Lemma get_spec_unary `{Inhab D} (x_ind x_val : loc) d 
   (k : int) 
   (* (Hk : (0 <= k < xind[(length xind - 1)])) *)
   (a : int) (Ha : (0 <= a < (length xind - 1))) 
   (Hka : (xind[a] <= k < xind[a + 1])) : 
   htriple (single d tt) 
-    (fun=> rli k x_ind x_val)
+    (fun=> get k x_ind x_val)
     (harray_int xind x_ind d \* 
       harray_int xval x_val d)
     (fun hr => 
@@ -67,10 +81,10 @@ Proof.
   xapp; xsimpl*.
 Qed.
 
-Lemma rli_spec_seg `{Inhab D} (x_ind x_val : loc) (k : int) 
+Lemma get_spec_seg `{Inhab D} (x_ind x_val : loc) (k : int) 
   (Hk : 0 <= k < (length xind - 1)) l : 
   htriple (label (Lab l (ind_seg xind k)))
-    (fun d => rli (eld d) x_ind x_val)
+    (fun d => get (eld d) x_ind x_val)
     ((\*_(d0 <- (label (Lab l (ind_seg xind k)))) 
         (harray_int xind x_ind d0 \* 
         harray_int xval x_val d0)))
@@ -93,20 +107,14 @@ Proof.
   rewrite indom_label_eq /ind_seg indom_interval in Hin. destruct Hin as (<- & Hin).
   rewrite -wp_equiv wp_single. 
   simpl.
-  xapp (@rli_spec_unary H x_ind x_val (Lab l d) d k Hk Hin)=> r Er.
+  xapp (@get_spec_unary H x_ind x_val (Lab l d) d k Hk Hin)=> r Er.
   rewrite Er.
   xsimpl*.
 Qed.
 
-End rli.
+End get.
 
 Section rlsum.
-
-Notation "'for' i <- '[' Z ',' N ']' '{' t '}'"  :=
-  (For Z N <{ fun_ i => t }>)
-  (in custom trm at level 69,
-    Z, N, i at level 0,
-    format "'[' for  i  <-  [ Z ','  N ] ']'  '{' '/   ' '[' t  '}' ']'") : trm_scope.
 
 Variables (M N : int).
 Hypotheses (EM : M = length xind - 1) (EN : N = xind[M]).
@@ -142,7 +150,7 @@ Lemma rlsum_spec `{Inhab D} (x_ind x_val : loc) :
      (\*_(i <- `[0, N]) arr(x_val, xval)⟨2, i⟩) }}
   [{
     [1| ld in `{0}   => rlsum x_ind x_val];
-    [2| ld in `[0,N] => rli ld x_ind x_val]
+    [2| ld in `[0,N] => get ld x_ind x_val]
   }]
   {{ hv, \[hv[`1](0) = Σ_(i <- `[0,N]) hv[`2](i)] \* 
       arr(x_ind, xind)⟨1, 0⟩ \*
@@ -164,7 +172,7 @@ Proof with fold'.
     rewrite /Inv /R /op.
     (xin (1,0): (do 9 (xwp; xapp)))...
     subst M.
-    xapp (@rli_spec_seg H x_ind x_val l0 H0)=> r.
+    xapp (@get_spec_seg H x_ind x_val l0 H0)=> r.
     rewrite hstar_fset_pure.
     xsimpl=> Er.
     (* TODO have no other way? can only touch himpl? *)
@@ -196,5 +204,152 @@ Qed.
 End rlsum.
 
 End runlength.
+
+Section alpha_blending.
+
+Import List.
+
+Context (xind xval : list int) {HindIIL : IncreasingIntList xind}.
+Hypothesis H_length_xval : length xval = length xind - 1 :> int.
+Hypothesis H_xval_notnil : 0 < length xval.
+
+Context (yind yval : list int) {HindIIL' : IncreasingIntList yind}.
+Hypothesis H_length_yval : length yval = length yind - 1 :> int.
+Hypothesis H_yval_notnil : 0 < length yval.
+
+Context (Mx My N : int).
+Hypotheses (EMx : Mx = length xind - 1) (ENx : N = xind[Mx]).
+Hypotheses (EMy : My = length yind - 1) (ENy : N = yind[My]).
+Hypotheses (xind0 : xind[0] = 0) (yind0 : yind[0] = 0).
+
+Context (α β : int).
+
+Notation "'i'"     := ("i":var) (in custom trm at level 0) : trm_scope.
+Notation "'iX'"     := ("iX":var) (in custom trm at level 0) : trm_scope.
+Notation "'iY'"     := ("iY":var) (in custom trm at level 0) : trm_scope.
+Notation "'iXl'"    := ("iXl":var) (in custom trm at level 0) : trm_scope.
+Notation "'iYl'"    := ("iYl":var) (in custom trm at level 0) : trm_scope.
+Notation "'ix'"     := ("ix":var) (in custom trm at level 0) : trm_scope.
+Notation "'iy'"     := ("iy":var) (in custom trm at level 0) : trm_scope.
+Notation "'ans'"    := ("ans":var) (in custom trm at level 0) : trm_scope.
+Notation "'step'"   := ("step":var) (in custom trm at level 0) : trm_scope.
+Notation "'stride'" := ("stride":var) (in custom trm at level 0) : trm_scope.
+Notation "'xindx'" := ("x_indx":var) (in custom trm at level 0) : trm_scope.
+Notation "'xvalx'" := ("x_valx":var) (in custom trm at level 0) : trm_scope.
+Notation "'yindy'" := ("y_indy":var) (in custom trm at level 0) : trm_scope.
+Notation "'yvaly'" := ("y_valy":var) (in custom trm at level 0) : trm_scope.
+Notation "'cnd'"    := ("cnd":var) (in custom trm at level 0) : trm_scope.
+Notation "'delta'"    := ("delta":var) (in custom trm at level 0) : trm_scope.
+
+Definition alpha_blend := <{
+  fun xind yind xval yval  =>
+    let ans    = ref 0 in
+    let iX     = ref 1 in
+    let iY     = ref 1 in
+    let step   = ref 0 in 
+    let stride = ref 0 in 
+      while (
+        let step = !step in 
+        step < N) {
+        let ix = !iX in 
+        let iy = !iY in 
+        let xindx = xind[ix] in 
+        let yindy = yind[iy] in 
+        let cnd = xindx = yindy in 
+          (if cnd then 
+            stride := xindx;
+            ++iX;
+            ++iY;
+            let step = !step in 
+            let stride = !stride in 
+            let delta = stride - step in 
+            let xvalx = xval[i] in 
+            let xvalx = α * xvalx in 
+            let yvaly = yval[i] in 
+            let yvaly = β * yvaly in 
+            let xvalx = xvalx + yvaly in 
+            let xvalx = xvalx * delta in
+              ans += xvalx
+          else 
+            let cnd = xindx < yindy in 
+            if cnd then 
+              stride := xindx;
+              ++iX;
+              let step = !step in 
+              let stride = !stride in 
+              let delta = stride - step in 
+              let xvalx = xval[i] in 
+              let xvalx = α * xvalx in 
+              let yvaly = yval[i] in 
+              let yvaly = β * yvaly in 
+              let xvalx = xvalx + yvaly in 
+              let xvalx = xvalx * delta in
+                ans += xvalx
+            else 
+              stride := yindy;
+              ++iY;
+              let step = !step in 
+              let stride = !stride in 
+              let delta = stride - step in 
+              let xvalx = xval[i] in 
+              let xvalx = α * xvalx in 
+              let yvaly = yval[i] in 
+              let yvaly = β * yvaly in 
+              let xvalx = xvalx + yvaly in 
+              let xvalx = xvalx * delta in
+                ans += xvalx);
+          let stride = !stride in
+          step := stride
+      }; !ans
+}>.
+
+Lemma lhtriple_free D : forall (p : loc) (v : val) fs,
+  @htriple D fs (fun d => val_free p)
+    (\*_(d <- fs) p ~(d)~> v)
+    (fun _ => \[]).
+Proof using. intros. apply htriple_free. Qed.
+
+Hint Resolve lhtriple_free : lhtriple.
+
+Notation "H1 '\\*' H2" := (hstar H1 H2)
+  (at level 42, right associativity, format "H1  \\* '//' H2") : hprop_scope.
+
+Lemma val_int_eq i j : 
+  (val_int i = val_int j) = (i = j).
+Proof. by extens; split=> [[]|]->. Qed.
+
+Ltac fold' := 
+  rewrite ?label_single ?wp_single ?val_int_eq
+    -/(While_aux _ _) 
+    -/(While _ _) //=; try lia.
+
+Lemma alpha_blend_spec `{Inhab (labeled int)} (x_ind x_val y_ind y_val : loc) : 
+  {{ (arr(x_ind, xind)⟨1, 0⟩ \* arr(y_ind, yind)⟨1, 0⟩ \*
+     arr(x_val, xval)⟨1, 0⟩ \* arr(y_val, yval)⟨1, 0⟩) \*
+     (\*_(i <- `[0, N]) arr(x_ind, xind)⟨2, i⟩) \\*
+     (\*_(i <- `[0, N]) arr(x_val, xval)⟨2, i⟩) \\* 
+     (\*_(i <- `[0, N]) arr(y_ind, yind)⟨3, i⟩) \\*
+     (\*_(i <- `[0, N]) arr(y_val, yval)⟨3, i⟩) }}
+  [{
+    {1| ld in `{0}   => alpha_blend x_ind y_ind x_val y_val};
+    {2| ld in `[0,N] => get ld x_ind x_val};
+    {3| ld in `[0,N] => get ld y_ind y_val}
+  }]
+  {{ hv, \[hv[`1](0) = Σ_(i <- `[0,N]) (α * hv[`2](i) + β * hv[`3](i))] 
+      \* \Top}}.
+Proof with fold'.
+  set (ind := merge xind yind).
+  have?: sorted xind by admit. 
+  have?: sorted yind by admit.
+  have?: NoDup xind by admit. 
+  have?: NoDup yind by admit.
+  have ndind: NoDup ind by exact/sorted_nodup/sorted_merge.
+  xin (1,0): (xwp;xapp=> ans); (xwp;xapp=> iX); 
+    (xwp;xapp=> iY); (xwp;xapp=> step); (xwp;xapp=> stride)...
+Admitted.
+
+
+End alpha_blending.
+
 
 End runlength.
